disk-betree/UI.dfy
@@ -1,0 +1,32 @@
+include "../lib/NativeTypes.dfy"
+
+module ValueWithDefault {
+  import NativeTypes
+
+  type Value(==,!new) = seq<NativeTypes.byte>
+	function method DefaultValue() : Value { [] }
+
+	export S provides Value, DefaultValue
+	export Internal reveals *
+	export extends S
+}
+
+module UI {
+  //import Keyspace = Total_Order
+  import Keyspace = Lexicographic_Byte_Order
+
+  import V = ValueWithDefault
+  type Key = Keyspace.Element
+  type Value = V.Value
+
+  datatype Op =
+    | NoOp
+    | SyncOp
+    | CrashOp
+    | PushSyncOp(id: int)
+    | PopSyncOp(id: int)
+
+    // TODO make these async? any value from it?
+    | GetOp(key: Key, value: Value)
+    | PutOp(key: Key, value: Value)
+}
