disk-betree/UIStateMachine.dfy
@@ -1,0 +1,11 @@
+include "UI.dfy"
+
+abstract module UIStateMachine {
+  import UI
+  type UIOp = UI.Op
+
+  type Constants
+  type Variables
+  predicate Init(k: Constants, s: Variables)
+  predicate Next(k: Constants, s: Variables, s': Variables, uiop: UIOp)
+}
